ContextAlgebra/theories/ResourceExtension.v
@@ -1,0 +1,1384 @@
+From ContextBase Require Import Prelude LogicVar BaseTactics.
+From ContextStore Require Import Store.
+From ContextAlgebra Require Import ResourceCore ResourceAlgebra.
+From Stdlib Require Import Logic.ProofIrrelevance.
+
+(** * Fiber extensions for abstract resources *)
+
+Section ResourceExtensionA.
+
+Context {K : Type} `{Countable K} .
+Context {V : Type} `{ValueSig V}.
+
+Local Notation StoreAT := (gmap K V) (only parsing).
+Local Notation WorldAT := (@WorldA K _ _ V) (only parsing).
+Local Notation WfWorldAT := (@WfWorldA K _ _ V) (only parsing).
+
+Record fiber_extensionA := {
+  extA_in : gset K;
+  extA_out : gset K;
+  extA_disjoint : extA_in ## extA_out;
+  extA_rel : StoreAT → WfWorldAT → Prop;
+
+  extA_rel_dom :
+    ∀ σ w,
+      dom σ = extA_in →
+      extA_rel σ w →
+      worldA_dom (w : WorldAT) = extA_out;
+
+  extA_rel_nonempty :
+    ∀ σ,
+      dom σ = extA_in →
+      ∃ w σe, extA_rel σ w ∧ (w : WorldAT) σe;
+
+  extA_rel_extensional :
+    ∀ σ w1 w2 σe,
+      dom σ = extA_in →
+      extA_rel σ w1 →
+      extA_rel σ w2 →
+      ((w1 : WorldAT) σe ↔ (w2 : WorldAT) σe);
+}.
+
+Definition mk_fiber_extensionA
+    (X Y : gset K) (R : StoreAT → WfWorldAT → Prop)
+    (Hdisj : X ## Y)
+    (Hdom : ∀ σ w, dom σ = X → R σ w → worldA_dom (w : WorldAT) = Y)
+    (Hne : ∀ σ, dom σ = X → ∃ w σe, R σ w ∧ (w : WorldAT) σe)
+    (Hext : ∀ σ w1 w2 σe,
+      dom σ = X → R σ w1 → R σ w2 →
+      ((w1 : WorldAT) σe ↔ (w2 : WorldAT) σe))
+    : fiber_extensionA :=
+  {| extA_in := X; extA_out := Y; extA_rel := R;
+     extA_disjoint := Hdisj; extA_rel_dom := Hdom;
+     extA_rel_nonempty := Hne; extA_rel_extensional := Hext |}.
+
+Definition fiber_extensionA_functional_on (m : WfWorldAT) (F : fiber_extensionA) : Prop :=
+  ∀ σ w σe1 σe2,
+    (m : WorldAT) σ →
+    extA_rel F (@storeA_restrict V K _ _ σ (extA_in F)) w →
+    (w : WorldAT) σe1 →
+    (w : WorldAT) σe2 →
+    σe1 = σe2.
+
+Record extension_applicableA (F : fiber_extensionA) (m : WfWorldAT) : Prop := {
+  extA_app_in : extA_in F ⊆ worldA_dom (m : WorldAT);
+  extA_app_out : extA_out F ## worldA_dom (m : WorldAT);
+}.
+
+Definition resA_extend_by (m : WfWorldAT) (F : fiber_extensionA) (n : WfWorldAT) : Prop :=
+  extension_applicableA F m ∧
+  worldA_dom (n : WorldAT) = worldA_dom (m : WorldAT) ∪ extA_out F ∧
+  ∀ σ,
+    (n : WorldAT) σ ↔
+      ∃ σm we σe,
+        (m : WorldAT) σm ∧
+        extA_rel F (@storeA_restrict V K _ _ σm (extA_in F)) we ∧
+        (we : WorldAT) σe ∧
+        σ = @union (gmap K V) _ σm σe.
+
+Notation "m '#>' F '~~A>' n" := (resA_extend_by m F n)
+  (at level 70, F at next level, n at next level).
+
+Definition fiber_extensionA_equiv_on (m : WfWorldAT) (F G : fiber_extensionA) : Prop :=
+  extA_in F = extA_in G ∧
+  ∀ σ wF wG σe,
+    (m : WorldAT) σ →
+    extA_rel F (@storeA_restrict V K _ _ σ (extA_in F)) wF →
+    extA_rel G (@storeA_restrict V K _ _ σ (extA_in G)) wG →
+    ((wF : WorldAT) σe ↔ (wG : WorldAT) σe).
+
+Lemma resA_extend_by_applicable m F n :
+  m #> F ~~A> n →
+  extension_applicableA F m.
+Proof. intros [Happ _]. exact Happ. Qed.
+
+Lemma resA_extend_by_dom m F n :
+  m #> F ~~A> n →
+  worldA_dom (n : WorldAT) = worldA_dom (m : WorldAT) ∪ extA_out F.
+Proof. intros [_ [Hdom _]]. exact Hdom. Qed.
+
+Lemma resA_extend_by_store_iff m F n σ :
+  m #> F ~~A> n →
+  (n : WorldAT) σ ↔
+    ∃ σm we σe,
+      (m : WorldAT) σm ∧
+      extA_rel F (@storeA_restrict V K _ _ σm (extA_in F)) we ∧
+      (we : WorldAT) σe ∧
+      σ = @union (gmap K V) _ σm σe.
+Proof. intros [_ [_ Hstores]]. exact (Hstores σ). Qed.
+
+Lemma extA_projection_dom m F σm :
+  extension_applicableA F m →
+  (m : WorldAT) σm →
+  dom (@storeA_restrict V K _ _ σm (extA_in F)) = extA_in F.
+Proof.
+  intros Happ Hσm.
+  transitivity (worldA_dom (m : WorldAT) ∩ extA_in F).
+  - rewrite <- (wfworldA_store_dom m σm Hσm).
+    apply storeA_restrict_dom.
+  - pose proof (extA_app_in _ _ Happ). set_solver.
+Qed.
+
+Lemma extA_output_store_dom F σ we σe :
+  dom (σ : gmap K V) = extA_in F →
+  extA_rel F σ we →
+  (we : WorldAT) σe →
+  dom (σe : gmap K V) = extA_out F.
+Proof.
+  intros Hdomσ HF Hσe.
+  pose proof (wfworldA_store_dom we σe Hσe) as Hdom_we.
+  change (dom (σe : gmap K V) = worldA_dom (we : WorldAT)) in Hdom_we.
+  rewrite Hdom_we.
+  eapply extA_rel_dom; eauto.
+Qed.
+
+Lemma extA_output_store_dom_from_base m F σm we σe :
+  extension_applicableA F m →
+  (m : WorldAT) σm →
+  extA_rel F (@storeA_restrict V K _ _ σm (extA_in F)) we →
+  (we : WorldAT) σe →
+  dom (σe : gmap K V) = extA_out F.
+Proof.
+  intros Happ Hσm HF Hσe.
+  eapply extA_output_store_dom; [| exact HF | exact Hσe].
+  eapply extA_projection_dom; eauto.
+Qed.
+
+Lemma resA_extend_store_compat m F σm we σe :
+  extension_applicableA F m →
+  (m : WorldAT) σm →
+  extA_rel F (@storeA_restrict V K _ _ σm (extA_in F)) we →
+  (we : WorldAT) σe →
+  @storeA_compat V K _ _ σm σe.
+Proof.
+  intros Happ Hσm HF Hσe.
+  apply storeA_disj_dom_compat.
+  change (dom (σm : gmap K V) ∩ dom (σe : gmap K V) = ∅).
+  pose proof (wfworldA_store_dom m σm Hσm) as Hdomσm.
+  change (dom (σm : gmap K V) = worldA_dom (m : WorldAT)) in Hdomσm.
+  assert (Hdomσe : dom (σe : gmap K V) = extA_out F).
+  { eapply extA_output_store_dom_from_base; eauto. }
+  rewrite Hdomσm, Hdomσe.
+  pose proof (extA_app_out _ _ Happ). set_solver.
+Qed.
+
+Lemma resA_extend_by_exists m F :
+  extension_applicableA F m →
+  ∃ n, m #> F ~~A> n.
+Proof.
+  intros Happ.
+  unshelve eexists.
+  - refine (exist _ {|
+      worldA_dom := worldA_dom (m : WorldAT) ∪ extA_out F;
+      worldA_stores := fun σ =>
+        exists σm we σe,
+          (m : WorldAT) σm /\
+          extA_rel F (@storeA_restrict V K _ _ σm (extA_in F)) we /\
+          (we : WorldAT) σe /\
+          σ = @union (gmap K V) _ σm σe
+    |} _).
+    constructor.
+    + destruct (worldA_wf m) as [Hne _].
+      destruct Hne as [σm Hσm].
+      assert (Hproj_dom :
+          dom (@storeA_restrict V K _ _ σm (extA_in F)) = extA_in F)
+        by (eapply extA_projection_dom; eauto).
+      destruct (extA_rel_nonempty F
+        (@storeA_restrict V K _ _ σm (extA_in F)) Hproj_dom)
+        as [we [σe [HF Hσe]]].
+      exists (@union (gmap K V) _ (σm : gmap K V) (σe : gmap K V)).
+      exists σm, we, σe. repeat split; eauto.
+    + intros σ [σm [we [σe [Hσm [HF [Hσe ->]]]]]].
+      transitivity (dom (σm : gmap K V) ∪ dom (σe : gmap K V)).
+      * apply storeA_union_dom.
+        eapply resA_extend_store_compat; eauto.
+      * pose proof (wfworldA_store_dom m σm Hσm) as Hdomσm.
+        pose proof (extA_output_store_dom_from_base m F σm we σe
+          Happ Hσm HF Hσe) as Hdomσe.
+        change (dom (σm : gmap K V) = worldA_dom (m : WorldAT)) in Hdomσm.
+        rewrite Hdomσm, Hdomσe.
+        set_solver.
+  - split; [exact Happ |].
+    split; [reflexivity |].
+    intros σ. reflexivity.
+Qed.
+
+Lemma resA_extend_by_unique m F n1 n2 :
+  m #> F ~~A> n1 →
+  m #> F ~~A> n2 →
+  n1 = n2.
+Proof.
+  intros H1 H2.
+  apply wfworldA_ext. apply worldA_ext.
+  - rewrite (resA_extend_by_dom _ _ _ H1).
+    rewrite (resA_extend_by_dom _ _ _ H2).
+    reflexivity.
+  - intros σ.
+    rewrite (resA_extend_by_store_iff _ _ _ σ H1).
+    rewrite (resA_extend_by_store_iff _ _ _ σ H2).
+    reflexivity.
+Qed.
+
+Lemma resA_extend_by_projection_eq m n F my ny :
+  resA_restrict m (extA_in F) = resA_restrict n (extA_in F) →
+  m #> F ~~A> my →
+  n #> F ~~A> ny →
+  resA_restrict my (extA_in F ∪ extA_out F) =
+  resA_restrict ny (extA_in F ∪ extA_out F).
+Proof.
+  intros Hproj Hmy Hny.
+  apply wfworldA_ext. apply worldA_ext.
+  - simpl.
+    rewrite (resA_extend_by_dom _ _ _ Hmy).
+    rewrite (resA_extend_by_dom _ _ _ Hny).
+    pose proof (resA_extend_by_applicable _ _ _ Hmy) as Happ_m.
+    pose proof (resA_extend_by_applicable _ _ _ Hny) as Happ_n.
+    pose proof (extA_app_in _ _ Happ_m) as Hin_m.
+    pose proof (extA_app_in _ _ Happ_n) as Hin_n.
+    pose proof (extA_app_out _ _ Happ_m) as Hout_m.
+    pose proof (extA_app_out _ _ Happ_n) as Hout_n.
+    set_solver.
+  - intros σ. split.
+    + intros [σmy [Hσmy Hrestrict]].
+      apply (proj1 (resA_extend_by_store_iff _ _ _ _ Hmy)) in Hσmy.
+      destruct Hσmy as [σm [we [σe [Hσm [HF [Hσe ->]]]]]].
+      assert (Hσm_proj :
+          (resA_restrict m (extA_in F) : WorldAT)
+            (@storeA_restrict V K _ _ σm (extA_in F))).
+      { exists σm. split; [exact Hσm | reflexivity]. }
+      rewrite Hproj in Hσm_proj.
+      destruct Hσm_proj as [σn [Hσn Hσn_proj]].
+      pose proof (extA_output_store_dom_from_base m F σm we σe
+        (resA_extend_by_applicable _ _ _ Hmy) Hσm HF Hσe) as Hdomσe.
+      exists (@union (gmap K V) _ (σn : gmap K V) (σe : gmap K V)).
+      split.
+      * apply (proj2 (resA_extend_by_store_iff _ _ _ _ Hny)).
+        exists σn, we, σe. repeat split; eauto.
+        rewrite Hσn_proj. exact HF.
+      * rewrite <- Hrestrict.
+        rewrite !storeA_restrict_union_cover.
+        -- rewrite Hσn_proj. reflexivity.
+        -- eapply (resA_extend_store_compat m F σm we σe); eauto.
+           exact (resA_extend_by_applicable _ _ _ Hmy).
+        -- pose proof (wfworldA_store_dom m σm Hσm) as Hdomσm.
+           change (dom (σm : gmap K V) = worldA_dom (m : WorldAT)) in Hdomσm.
+           rewrite Hdomσm.
+           exact (extA_app_in _ _ (resA_extend_by_applicable _ _ _ Hmy)).
+        -- rewrite Hdomσe. set_solver.
+        -- eapply (resA_extend_store_compat n F σn we σe).
+           ++ exact (resA_extend_by_applicable _ _ _ Hny).
+           ++ exact Hσn.
+           ++ rewrite Hσn_proj. exact HF.
+           ++ exact Hσe.
+        -- pose proof (wfworldA_store_dom n σn Hσn) as Hdomσn.
+           change (dom (σn : gmap K V) = worldA_dom (n : WorldAT)) in Hdomσn.
+           rewrite Hdomσn.
+           exact (extA_app_in _ _ (resA_extend_by_applicable _ _ _ Hny)).
+        -- rewrite Hdomσe. set_solver.
+    + intros [σny [Hσny Hrestrict]].
+      apply (proj1 (resA_extend_by_store_iff _ _ _ _ Hny)) in Hσny.
+      destruct Hσny as [σn [we [σe [Hσn [HF [Hσe ->]]]]]].
+      assert (Hσn_proj :
+          (resA_restrict n (extA_in F) : WorldAT)
+            (@storeA_restrict V K _ _ σn (extA_in F))).
+      { exists σn. split; [exact Hσn | reflexivity]. }
+      rewrite <- Hproj in Hσn_proj.
+      destruct Hσn_proj as [σm [Hσm Hσm_proj]].
+      pose proof (extA_output_store_dom_from_base n F σn we σe
+        (resA_extend_by_applicable _ _ _ Hny) Hσn HF Hσe) as Hdomσe.
+      exists (@union (gmap K V) _ (σm : gmap K V) (σe : gmap K V)).
+      split.
+      * apply (proj2 (resA_extend_by_store_iff _ _ _ _ Hmy)).
+        exists σm, we, σe. repeat split; eauto.
+        rewrite Hσm_proj. exact HF.
+      * rewrite <- Hrestrict.
+        rewrite !storeA_restrict_union_cover.
+        -- rewrite Hσm_proj. reflexivity.
+        -- eapply (resA_extend_store_compat n F σn we σe); eauto.
+           exact (resA_extend_by_applicable _ _ _ Hny).
+        -- pose proof (wfworldA_store_dom n σn Hσn) as Hdomσn.
+           change (dom (σn : gmap K V) = worldA_dom (n : WorldAT)) in Hdomσn.
+           rewrite Hdomσn.
+           exact (extA_app_in _ _ (resA_extend_by_applicable _ _ _ Hny)).
+        -- rewrite Hdomσe. set_solver.
+        -- eapply (resA_extend_store_compat m F σm we σe).
+           ++ exact (resA_extend_by_applicable _ _ _ Hmy).
+           ++ exact Hσm.
+           ++ rewrite Hσm_proj. exact HF.
+           ++ exact Hσe.
+        -- pose proof (wfworldA_store_dom m σm Hσm) as Hdomσm.
+           change (dom (σm : gmap K V) = worldA_dom (m : WorldAT)) in Hdomσm.
+           rewrite Hdomσm.
+           exact (extA_app_in _ _ (resA_extend_by_applicable _ _ _ Hmy)).
+        -- rewrite Hdomσe. set_solver.
+Qed.
+
+Lemma resA_extend_by_restrict_base m F n :
+  m #> F ~~A> n →
+  resA_restrict n (worldA_dom (m : WorldAT)) = m.
+Proof.
+  intros Hext.
+  destruct Hext as [Happ [Hdom_n Hstores]].
+  apply wfworldA_ext. apply worldA_ext.
+  - simpl. rewrite Hdom_n.
+    pose proof (extA_app_out _ _ Happ). set_solver.
+  - intros σ. split.
+    + intros [σn [Hσn Hrestrict]].
+      rewrite Hstores in Hσn.
+      destruct Hσn as [σm [we [σe [Hσm [HF [Hσe ->]]]]]].
+      pose proof (resA_extend_store_compat m F σm we σe Happ Hσm HF Hσe)
+        as Hcompat.
+      pose proof (wfworldA_store_dom m σm Hσm) as Hdomσm.
+      change (dom (σm : gmap K V) = worldA_dom (m : WorldAT)) in Hdomσm.
+      pose proof (extA_output_store_dom_from_base m F σm we σe
+        Happ Hσm HF Hσe) as Hdomσe.
+      assert (Hpiece :
+          @storeA_restrict V K _ _ (@union (gmap K V) _ σm σe)
+            (worldA_dom (m : WorldAT)) = σm).
+      {
+        apply (storeA_restrict_union_piece_l σm σe
+          (worldA_dom (m : WorldAT)) (extA_out F)).
+        - exact Hcompat.
+        - change (dom (σm : gmap K V) ⊆ worldA_dom (m : WorldAT)).
+          rewrite Hdomσm. reflexivity.
+        - change (dom (σe : gmap K V) ⊆ extA_out F).
+          rewrite Hdomσe. reflexivity.
+        - pose proof (extA_app_out _ _ Happ). set_solver.
+      }
+      rewrite Hpiece in Hrestrict. subst. exact Hσm.
+    + intros Hσ.
+      pose proof (wfworldA_store_dom m σ Hσ) as Hdomσ.
+      change (dom (σ : gmap K V) = worldA_dom (m : WorldAT)) in Hdomσ.
+      assert (Hproj_dom :
+          dom (@storeA_restrict V K _ _ σ (extA_in F)) = extA_in F)
+        by (eapply extA_projection_dom; eauto).
+      destruct (extA_rel_nonempty F
+        (@storeA_restrict V K _ _ σ (extA_in F)) Hproj_dom)
+        as [we [σe [HF Hσe]]].
+      exists (@union (gmap K V) _ (σ : gmap K V) (σe : gmap K V)).
+      split.
+      * rewrite Hstores.
+        exists σ, we, σe. repeat split; eauto.
+      * pose proof (resA_extend_store_compat m F σ we σe Happ Hσ HF Hσe)
+          as Hcompat.
+        pose proof (extA_output_store_dom_from_base m F σ we σe
+          Happ Hσ HF Hσe) as Hdomσe.
+        apply (storeA_restrict_union_piece_l σ σe
+          (worldA_dom (m : WorldAT)) (extA_out F)).
+        -- exact Hcompat.
+        -- change (dom (σ : gmap K V) ⊆ worldA_dom (m : WorldAT)).
+           rewrite Hdomσ. reflexivity.
+        -- change (dom (σe : gmap K V) ⊆ extA_out F).
+           rewrite Hdomσe. reflexivity.
+        -- pose proof (extA_app_out _ _ Happ). set_solver.
+Qed.
+
+Lemma resA_extend_by_le m F n :
+  m #> F ~~A> n →
+  m ⊑ n.
+Proof.
+  intros Hext.
+  unfold sqsubseteq, wf_worldA_sqsubseteq, resA_le, rawA_le.
+  change ((m : WorldAT) = rawA_restrict n (worldA_dom (m : WorldAT))).
+  exact (f_equal (fun w : WfWorldAT => (w : WorldAT))
+    (eq_sym (resA_extend_by_restrict_base m F n Hext))).
+Qed.
+
+Lemma resA_extend_store_restrict_base m F σm we σe :
+  extension_applicableA F m →
+  (m : WorldAT) σm →
+  extA_rel F (@storeA_restrict V K _ _ σm (extA_in F)) we →
+  (we : WorldAT) σe →
+  @storeA_restrict V K _ _ (@union (gmap K V) _ σm σe)
+    (worldA_dom (m : WorldAT)) = σm.
+Proof.
+  intros Happ Hσm HF Hσe.
+  pose proof (resA_extend_store_compat m F σm we σe Happ Hσm HF Hσe)
+    as Hcompat.
+  pose proof (wfworldA_store_dom m σm Hσm) as Hdomσm.
+  change (dom (σm : gmap K V) = worldA_dom (m : WorldAT)) in Hdomσm.
+  pose proof (extA_output_store_dom_from_base m F σm we σe
+    Happ Hσm HF Hσe) as Hdomσe.
+  apply (storeA_restrict_union_piece_l σm σe
+    (worldA_dom (m : WorldAT)) (extA_out F)).
+  - exact Hcompat.
+  - change (dom (σm : gmap K V) ⊆ worldA_dom (m : WorldAT)).
+    rewrite Hdomσm. reflexivity.
+  - change (dom (σe : gmap K V) ⊆ extA_out F).
+    rewrite Hdomσe. reflexivity.
+	  - pose proof (extA_app_out _ _ Happ). set_solver.
+Qed.
+
+Lemma resA_extend_by_slice_restrict_base
+    (m : WfWorldAT) F (n p : WfWorldAT)
+    (Hsub : resA_subset p (resA_restrict n (worldA_dom (m : WorldAT)))) :
+  m #> F ~~A> n →
+  worldA_dom (p : WorldAT) = worldA_dom (m : WorldAT) →
+  resA_subset p m →
+  p #> F ~~A> resA_slice_restrict n (worldA_dom (m : WorldAT)) p Hsub.
+Proof.
+  intros Hext Hdom_p Hsub_p_m.
+  pose proof (resA_extend_by_applicable _ _ _ Hext) as Happ.
+  split.
+  - constructor.
+    + rewrite Hdom_p. exact (extA_app_in _ _ Happ).
+    + rewrite Hdom_p. exact (extA_app_out _ _ Happ).
+  - split.
+    + simpl. rewrite (resA_extend_by_dom _ _ _ Hext), Hdom_p. reflexivity.
+    + intros σ. split.
+      * intros [Hσn Hσp].
+      apply (proj1 (resA_extend_by_store_iff _ _ _ _ Hext)) in Hσn.
+      destruct Hσn as [σm [we [σe [Hσm [HFrel [Hσe ->]]]]]].
+      exists σm, we, σe. repeat split; eauto.
+      replace σm with (@storeA_restrict V K _ _
+        (@union (gmap K V) _ σm σe) (worldA_dom (m : WorldAT))).
+      -- exact Hσp.
+      -- exact (resA_extend_store_restrict_base m F σm we σe
+          Happ Hσm HFrel Hσe).
+      * intros [σp [we [σe [Hσp [HFrel [Hσe ->]]]]]].
+      split.
+      -- apply (proj2 (resA_extend_by_store_iff _ _ _ _ Hext)).
+        exists σp, we, σe. repeat split; eauto.
+        exact (proj2 Hsub_p_m σp Hσp).
+      -- pose proof (proj2 Hsub_p_m σp Hσp) as Hσm.
+        rewrite (resA_extend_store_restrict_base m F σp we σe
+          Happ Hσm HFrel Hσe).
+        exact Hσp.
+Qed.
+
+Lemma resA_extend_store_restrict_other_input m F G σm we σe :
+  extension_applicableA F m →
+  extension_applicableA G m →
+  (m : WorldAT) σm →
+  extA_rel F (@storeA_restrict V K _ _ σm (extA_in F)) we →
+  (we : WorldAT) σe →
+  @storeA_restrict V K _ _ (@union (gmap K V) _ σm σe)
+    (extA_in G) =
+  @storeA_restrict V K _ _ σm (extA_in G).
+Proof.
+  intros HappF HappG Hσm HF Hσe.
+  apply storeA_restrict_union_ignore_r.
+  rewrite (extA_output_store_dom_from_base m F σm we σe
+    HappF Hσm HF Hσe).
+  pose proof (extA_app_in _ _ HappG).
+  pose proof (extA_app_out _ _ HappF).
+  set_solver.
+Qed.
+
+Lemma resA_extend_by_base_le m n F my ny :
+  m ⊑ n →
+  m #> F ~~A> my →
+  n #> F ~~A> ny →
+  my ⊑ ny.
+Proof.
+  intros Hmn Hmy Hny.
+  pose proof (rawA_le_dom m n Hmn) as Hdom_mn.
+  pose proof (resA_extend_by_applicable _ _ _ Hmy) as Happ_m.
+  pose proof (resA_extend_by_applicable _ _ _ Hny) as Happ_n.
+  unfold sqsubseteq, wf_worldA_sqsubseteq, resA_le, rawA_le.
+  apply worldA_ext.
+  - rewrite (resA_extend_by_dom _ _ _ Hmy).
+    simpl. rewrite (resA_extend_by_dom _ _ _ Hny). set_solver.
+  - intros σ. split.
+    + intros Hσmy.
+      apply (proj1 (resA_extend_by_store_iff _ _ _ _ Hmy)) in Hσmy.
+      destruct Hσmy as [σm [we [σe [Hσm [HF [Hσe ->]]]]]].
+      assert (Hσn_restricted : rawA_restrict n (worldA_dom (m : WorldAT)) σm).
+      {
+        change ((rawA_restrict n (worldA_dom (m : WorldAT)) : WorldAT) σm).
+        rewrite <- Hmn. exact Hσm.
+      }
+      destruct Hσn_restricted as [σn [Hσn Hrestrict_m]].
+      assert (HF_n :
+          extA_rel F (@storeA_restrict V K _ _ σn (extA_in F)) we).
+      {
+        replace (@storeA_restrict V K _ _ σn (extA_in F))
+          with (@storeA_restrict V K _ _ σm (extA_in F)); [exact HF |].
+        subst σm.
+        rewrite storeA_restrict_twice_subset; [reflexivity |].
+        exact (extA_app_in _ _ Happ_m).
+      }
+      exists (@union (gmap K V) _ (σn : gmap K V) (σe : gmap K V)).
+      split.
+      * apply (proj2 (resA_extend_by_store_iff _ _ _ _ Hny)).
+        exists σn, we, σe. repeat split; eauto.
+      * assert (Hcompat :
+            @storeA_compat V K _ _ σn σe).
+        { eapply resA_extend_store_compat; eauto. }
+        pose proof (wfworldA_store_dom n σn Hσn) as Hdomσn.
+        change (dom (σn : gmap K V) = worldA_dom (n : WorldAT)) in Hdomσn.
+        pose proof (extA_output_store_dom_from_base n F σn we σe
+          Happ_n Hσn HF_n Hσe) as Hdomσe_out.
+        rewrite (resA_extend_by_dom _ _ _ Hmy).
+        rewrite (storeA_restrict_union_cover σn σe
+          (worldA_dom (m : WorldAT)) (extA_out F)); eauto.
+        -- rewrite Hrestrict_m.
+           rewrite storeA_restrict_idemp; [reflexivity |].
+           rewrite Hdomσe_out. set_solver.
+        -- rewrite Hdomσn. exact Hdom_mn.
+        -- rewrite Hdomσe_out. set_solver.
+    + intros [σny [Hσny Hrestrict]].
+      apply (proj1 (resA_extend_by_store_iff _ _ _ _ Hny)) in Hσny.
+      destruct Hσny as [σn [we [σe [Hσn [HF [Hσe ->]]]]]].
+      assert (Hσm : (m : WorldAT)
+          (@storeA_restrict V K _ _ σn (worldA_dom (m : WorldAT)))).
+      {
+        assert (Hraw : (rawA_restrict n (worldA_dom (m : WorldAT)) : WorldAT)
+          (@storeA_restrict V K _ _ σn (worldA_dom (m : WorldAT)))).
+        { exists σn. split; [exact Hσn | reflexivity]. }
+        rewrite <- Hmn in Hraw. exact Hraw.
+      }
+      assert (HF_m :
+          extA_rel F (@storeA_restrict V K _ _
+            (@storeA_restrict V K _ _ σn (worldA_dom (m : WorldAT)))
+            (extA_in F)) we).
+      {
+        rewrite storeA_restrict_twice_subset; [exact HF |].
+        exact (extA_app_in _ _ Happ_m).
+      }
+      apply (proj2 (resA_extend_by_store_iff _ _ _ _ Hmy)).
+      exists (@storeA_restrict V K _ _ σn (worldA_dom (m : WorldAT))), we, σe.
+      repeat split; eauto.
+      assert (Hcompat :
+          @storeA_compat V K _ _ σn σe).
+      { eapply resA_extend_store_compat; eauto. }
+      pose proof (wfworldA_store_dom n σn Hσn) as Hdomσn.
+      change (dom (σn : gmap K V) = worldA_dom (n : WorldAT)) in Hdomσn.
+      pose proof (extA_output_store_dom_from_base n F σn we σe
+        Happ_n Hσn HF Hσe) as Hdomσe_out.
+      rewrite (resA_extend_by_dom _ _ _ Hmy) in Hrestrict.
+      rewrite (storeA_restrict_union_cover σn σe
+        (worldA_dom (m : WorldAT)) (extA_out F)) in Hrestrict; eauto.
+      * rewrite (storeA_restrict_idemp σe (extA_out F)) in Hrestrict;
+          [symmetry; exact Hrestrict |].
+        rewrite Hdomσe_out. set_solver.
+      * rewrite Hdomσn. exact Hdom_mn.
+      * rewrite Hdomσe_out. set_solver.
+Qed.
+
+End ResourceExtensionA.
+
+
+(** * Fiber extension equivalence and commuting lemmas *)
+
+
+Section ResourceExtensionA.
+
+Context {K : Type} `{Countable K} .
+Context {V : Type} `{ValueSig V}.
+
+Local Notation StoreAT := (gmap K V) (only parsing).
+Local Notation WorldAT := (@WorldA K _ _ V) (only parsing).
+Local Notation WfWorldAT := (@WfWorldA K _ _ V) (only parsing).
+Local Notation fiber_extensionA := (@fiber_extensionA K _ _ V).
+
+Local Notation "m '#>' F '~~A>' n" := (resA_extend_by m F n)
+  (at level 70, F at next level, n at next level).
+
+Lemma fiber_extensionA_functional_outputs_eq
+    (m : WfWorldAT) (F : fiber_extensionA)
+    (σ : StoreAT) (w1 w2 : WfWorldAT) (σe1 σe2 : StoreAT) :
+  extension_applicableA F m →
+  fiber_extensionA_functional_on m F →
+  (m : WorldAT) σ →
+  extA_rel F (@storeA_restrict V K _ _ σ (extA_in F)) w1 →
+  extA_rel F (@storeA_restrict V K _ _ σ (extA_in F)) w2 →
+  (w1 : WorldAT) σe1 →
+  (w2 : WorldAT) σe2 →
+  σe1 = σe2.
+Proof.
+  intros Happ Hfun Hσ Hw1 Hw2 Hσe1 Hσe2.
+  assert (Hproj_dom :
+      dom (@storeA_restrict V K _ _ σ (extA_in F)) = extA_in F)
+    by (eapply extA_projection_dom; eauto).
+  pose proof (proj1 (extA_rel_extensional F
+    (@storeA_restrict V K _ _ σ (extA_in F)) w1 w2 σe1
+    Hproj_dom Hw1 Hw2) Hσe1) as Hσe1_w2.
+  eapply Hfun; eauto.
+Qed.
+
+Lemma resA_extend_by_output_unique
+    (m : WfWorldAT) (F G : fiber_extensionA) (n : WfWorldAT) :
+  m #> F ~~A> n →
+  m #> G ~~A> n →
+  extA_out F = extA_out G.
+Proof.
+  intros HF HG.
+  pose proof (resA_extend_by_dom _ _ _ HF) as HFdom.
+  pose proof (resA_extend_by_dom _ _ _ HG) as HGdom.
+  pose proof (extA_app_out _ _ (resA_extend_by_applicable _ _ _ HF)) as HFfresh.
+  pose proof (extA_app_out _ _ (resA_extend_by_applicable _ _ _ HG)) as HGfresh.
+  set_solver.
+Qed.
+
+Lemma resA_extend_by_fiber_equiv_on
+    (m : WfWorldAT) (F G : fiber_extensionA) (n : WfWorldAT) :
+  extA_in F = extA_in G →
+  m #> F ~~A> n →
+  m #> G ~~A> n →
+  fiber_extensionA_equiv_on m F G.
+Proof.
+  intros Hin HF HG. split; [exact Hin |].
+  assert (Hdir :
+    forall A B,
+      extA_in A = extA_in B ->
+      m #> A ~~A> n ->
+      m #> B ~~A> n ->
+      forall σ wA wB σe,
+        (m : WorldAT) σ ->
+        extA_rel A (@storeA_restrict V K _ _ σ (extA_in A)) wA ->
+        extA_rel B (@storeA_restrict V K _ _ σ (extA_in B)) wB ->
+        (wA : WorldAT) σe ->
+        (wB : WorldAT) σe).
+  {
+    intros A B HAB HA HB σ wA wB σe Hσ HArel HBrel HAe.
+    pose proof (resA_extend_by_applicable _ _ _ HA) as HAppA.
+    pose proof (resA_extend_by_applicable _ _ _ HB) as HAppB.
+    pose proof (resA_extend_store_compat m A σ wA σe HAppA Hσ HArel HAe)
+      as HcompatA.
+    assert (Hn : (n : WorldAT) (@union (gmap K V) _ σ σe)).
+    {
+      apply (proj2 (resA_extend_by_store_iff m A n
+        (@union (gmap K V) _ σ σe) HA)).
+      exists σ, wA, σe. repeat split; eauto.
+    }
+    apply (proj1 (resA_extend_by_store_iff m B n
+      (@union (gmap K V) _ σ σe) HB)) in Hn.
+    destruct Hn as [σB [wBe [σBe [HσB [HBwe [HBe Heq]]]]]].
+    pose proof (resA_extend_store_compat m B σB wBe σBe HAppB HσB HBwe HBe)
+      as HcompatB.
+    assert (Hdomσ : dom (σ : gmap K V) = worldA_dom (m : WorldAT)).
+    { exact (wfworldA_store_dom m σ Hσ). }
+    assert (HdomσB : dom (σB : gmap K V) = worldA_dom (m : WorldAT)).
+    { exact (wfworldA_store_dom m σB HσB). }
+    assert (HprojA :
+        dom (@storeA_restrict V K _ _ σ (extA_in A)) = extA_in A)
+      by (eapply extA_projection_dom; eauto).
+    assert (HprojB :
+        dom (@storeA_restrict V K _ _ σB (extA_in B)) = extA_in B)
+      by (eapply extA_projection_dom; eauto).
+    assert (Hdomσe : dom (σe : gmap K V) = extA_out A).
+    {
+      pose proof (wfworldA_store_dom wA σe HAe) as Hdom_wA.
+      change (dom (σe : gmap K V) = worldA_dom (wA : WorldAT)) in Hdom_wA.
+      rewrite Hdom_wA. eapply extA_rel_dom; eauto.
+    }
+    assert (HdomσBe : dom (σBe : gmap K V) = extA_out B).
+    {
+      pose proof (wfworldA_store_dom wBe σBe HBe) as Hdom_wBe.
+      change (dom (σBe : gmap K V) = worldA_dom (wBe : WorldAT)) in Hdom_wBe.
+      rewrite Hdom_wBe. eapply extA_rel_dom; eauto.
+    }
+    pose proof (resA_extend_by_output_unique m A B n HA HB) as Hout.
+    assert (HbaseA :
+        @storeA_restrict V K _ _ (@union (gmap K V) _ σ σe)
+          (worldA_dom (m : WorldAT)) = σ).
+    {
+      apply (storeA_restrict_union_piece_l σ σe
+        (worldA_dom (m : WorldAT)) (extA_out A)); eauto.
+      - change (dom (σ : gmap K V) ⊆ worldA_dom (m : WorldAT)).
+        rewrite Hdomσ. reflexivity.
+      - change (dom (σe : gmap K V) ⊆ extA_out A).
+        rewrite Hdomσe. reflexivity.
+      - pose proof (extA_app_out _ _ HAppA). set_solver.
+    }
+    assert (HbaseB :
+        @storeA_restrict V K _ _ (@union (gmap K V) _ σB σBe)
+          (worldA_dom (m : WorldAT)) = σB).
+    {
+      apply (storeA_restrict_union_piece_l σB σBe
+        (worldA_dom (m : WorldAT)) (extA_out B)); eauto.
+      - change (dom (σB : gmap K V) ⊆ worldA_dom (m : WorldAT)).
+        rewrite HdomσB. reflexivity.
+      - change (dom (σBe : gmap K V) ⊆ extA_out B).
+        rewrite HdomσBe. reflexivity.
+      - pose proof (extA_app_out _ _ HAppB). set_solver.
+    }
+    assert (HσB_eq : σB = σ).
+    {
+      rewrite <- Heq in HbaseB.
+      rewrite HbaseA in HbaseB. symmetry. exact HbaseB.
+    }
+    subst σB.
+    assert (HextraA :
+        @storeA_restrict V K _ _ (@union (gmap K V) _ σ σe) (extA_out A) = σe).
+    {
+      apply (storeA_restrict_union_piece_r σ σe
+        (worldA_dom (m : WorldAT)) (extA_out A)); eauto.
+      - change (dom (σ : gmap K V) ⊆ worldA_dom (m : WorldAT)).
+        rewrite Hdomσ. reflexivity.
+      - change (dom (σe : gmap K V) ⊆ extA_out A).
+        rewrite Hdomσe. reflexivity.
+      - pose proof (extA_app_out _ _ HAppA). set_solver.
+    }
+    assert (HextraB :
+        @storeA_restrict V K _ _ (@union (gmap K V) _ σ σBe) (extA_out B) = σBe).
+    {
+      apply (storeA_restrict_union_piece_r σ σBe
+        (worldA_dom (m : WorldAT)) (extA_out B)); eauto.
+      - change (dom (σ : gmap K V) ⊆ worldA_dom (m : WorldAT)).
+        rewrite Hdomσ. reflexivity.
+      - change (dom (σBe : gmap K V) ⊆ extA_out B).
+        rewrite HdomσBe. reflexivity.
+      - pose proof (extA_app_out _ _ HAppB). set_solver.
+    }
+    assert (HσBe_eq : σBe = σe).
+    {
+      rewrite <- Heq in HextraB.
+      rewrite <- Hout in HextraB.
+      rewrite HextraA in HextraB. symmetry. exact HextraB.
+    }
+    subst σBe.
+    replace (@storeA_restrict V K _ _ σ (extA_in A))
+      with (@storeA_restrict V K _ _ σ (extA_in B)) in HBwe
+      by (rewrite HAB; reflexivity).
+    replace (@storeA_restrict V K _ _ σ (extA_in A))
+      with (@storeA_restrict V K _ _ σ (extA_in B)) in HBrel
+      by (rewrite HAB; reflexivity).
+    apply (proj1 (extA_rel_extensional B
+      (@storeA_restrict V K _ _ σ (extA_in B)) wBe wB σe
+      HprojB HBwe HBrel)).
+    exact HBe.
+  }
+  intros σ wF wG σe Hσ HFrel HGrel. split.
+  - eapply Hdir; eauto.
+  - intros HGe.
+    eapply Hdir with (A := G) (B := F) (σ := σ) (wA := wG) (wB := wF); eauto;
+      symmetry; exact Hin.
+Qed.
+
+Lemma resA_extend_by_commute
+    (m : WfWorldAT) (F G : fiber_extensionA)
+    (mF mG mFG mGF : WfWorldAT) :
+  m #> F ~~A> mF →
+  m #> G ~~A> mG →
+  mF #> G ~~A> mFG →
+  mG #> F ~~A> mGF →
+  mFG = mGF.
+Proof.
+  intros HF HG HFG HGF.
+  pose proof (resA_extend_by_dom _ _ _ HF) as Hdom_mF.
+  pose proof (resA_extend_by_dom _ _ _ HG) as Hdom_mG.
+  pose proof (resA_extend_by_applicable _ _ _ HF) as HAppF_m.
+  pose proof (resA_extend_by_applicable _ _ _ HG) as HAppG_m.
+  pose proof (resA_extend_by_applicable _ _ _ HFG) as HAppG_mF.
+  pose proof (resA_extend_by_applicable _ _ _ HGF) as HAppF_mG.
+  pose proof (extA_app_out _ _ HAppF_m) as HFfresh_m.
+  pose proof (extA_app_out _ _ HAppG_m) as HGfresh_m.
+  pose proof (extA_app_out _ _ HAppG_mF) as HGfresh_mF.
+  pose proof (extA_app_out _ _ HAppF_mG) as HFfresh_mG.
+  assert (HFGfresh : extA_out F ## extA_out G) by set_solver.
+  assert (HGFfresh : extA_out G ## extA_out F) by set_solver.
+  apply wfworldA_ext. apply worldA_ext.
+  - rewrite (resA_extend_by_dom _ _ _ HFG).
+    rewrite (resA_extend_by_dom _ _ _ HGF).
+    rewrite Hdom_mF, Hdom_mG. set_solver.
+  - intros σ. split.
+    + intros Hσ.
+      apply (proj2 (resA_extend_by_store_iff _ _ _ _ HGF)).
+      apply (proj1 (resA_extend_by_store_iff _ _ _ _ HFG)) in Hσ.
+      destruct Hσ as [σmF [wG [σge [HmFσ [HGrel [HGstore ->]]]]]].
+      apply (proj1 (resA_extend_by_store_iff _ _ _ _ HF)) in HmFσ.
+      destruct HmFσ as [σm [wF [σfe [Hmσ [HFrel [HFstore ->]]]]]].
+      pose proof (resA_extend_store_compat m F σm wF σfe
+        HAppF_m Hmσ HFrel HFstore) as HcompatF.
+      pose proof (extA_output_store_dom_from_base m F σm wF σfe
+        HAppF_m Hmσ HFrel HFstore) as Hdomσfe.
+      assert (HprojG :
+          @storeA_restrict V K _ _ (@union (gmap K V) _ σm σfe) (extA_in G) =
+          @storeA_restrict V K _ _ σm (extA_in G)).
+      {
+        exact (resA_extend_store_restrict_other_input m F G σm wF σfe
+          HAppF_m HAppG_m Hmσ HFrel HFstore).
+      }
+      rewrite HprojG in HGrel.
+      pose proof (resA_extend_store_compat m G σm wG σge
+        HAppG_m Hmσ HGrel HGstore) as HcompatG.
+      pose proof (extA_output_store_dom_from_base m G σm wG σge
+        HAppG_m Hmσ HGrel HGstore) as Hdomσge.
+      exists (@union (gmap K V) _ (σm : gmap K V) (σge : gmap K V)), wF, σfe.
+      split.
+      * apply (proj2 (resA_extend_by_store_iff _ _ _ _ HG)).
+        exists σm, wG, σge. repeat split; eauto.
+      * split.
+        -- assert (HprojF :
+             @storeA_restrict V K _ _
+               (@union (gmap K V) _ σm σge) (extA_in F) =
+             @storeA_restrict V K _ _ σm (extA_in F)).
+           {
+             exact (resA_extend_store_restrict_other_input m G F σm wG σge
+               HAppG_m HAppF_m Hmσ HGrel HGstore).
+           }
+           rewrite HprojF. exact HFrel.
+        -- split; [exact HFstore |].
+           assert (Hcompat_extra : @storeA_compat V K _ _ σfe σge).
+           {
+             apply storeA_disj_dom_compat.
+             change (dom (σfe : gmap K V) ∩ dom (σge : gmap K V) = ∅).
+             rewrite Hdomσfe, Hdomσge. set_solver.
+           }
+           apply storeA_union_swap_right. exact Hcompat_extra.
+    + intros Hσ.
+      apply (proj2 (resA_extend_by_store_iff _ _ _ _ HFG)).
+      apply (proj1 (resA_extend_by_store_iff _ _ _ _ HGF)) in Hσ.
+      destruct Hσ as [σmG [wF [σfe [HmGσ [HFrel [HFstore ->]]]]]].
+      apply (proj1 (resA_extend_by_store_iff _ _ _ _ HG)) in HmGσ.
+      destruct HmGσ as [σm [wG [σge [Hmσ [HGrel [HGstore ->]]]]]].
+      pose proof (resA_extend_store_compat m G σm wG σge
+        HAppG_m Hmσ HGrel HGstore) as HcompatG.
+      pose proof (extA_output_store_dom_from_base m G σm wG σge
+        HAppG_m Hmσ HGrel HGstore) as Hdomσge.
+      assert (HprojF :
+          @storeA_restrict V K _ _ (@union (gmap K V) _ σm σge) (extA_in F) =
+          @storeA_restrict V K _ _ σm (extA_in F)).
+      {
+        exact (resA_extend_store_restrict_other_input m G F σm wG σge
+          HAppG_m HAppF_m Hmσ HGrel HGstore).
+      }
+      rewrite HprojF in HFrel.
+      pose proof (resA_extend_store_compat m F σm wF σfe
+        HAppF_m Hmσ HFrel HFstore) as HcompatF.
+      pose proof (extA_output_store_dom_from_base m F σm wF σfe
+        HAppF_m Hmσ HFrel HFstore) as Hdomσfe.
+      exists (@union (gmap K V) _ (σm : gmap K V) (σfe : gmap K V)), wG, σge.
+      split.
+      * apply (proj2 (resA_extend_by_store_iff _ _ _ _ HF)).
+        exists σm, wF, σfe. repeat split; eauto.
+      * split.
+        -- assert (HprojG :
+             @storeA_restrict V K _ _
+               (@union (gmap K V) _ σm σfe) (extA_in G) =
+             @storeA_restrict V K _ _ σm (extA_in G)).
+           {
+             exact (resA_extend_store_restrict_other_input m F G σm wF σfe
+               HAppF_m HAppG_m Hmσ HFrel HFstore).
+           }
+           rewrite HprojG. exact HGrel.
+        -- split; [exact HGstore |].
+           assert (Hcompat_extra : @storeA_compat V K _ _ σge σfe).
+           {
+             apply storeA_disj_dom_compat.
+             change (dom (σge : gmap K V) ∩ dom (σfe : gmap K V) = ∅).
+             rewrite Hdomσge, Hdomσfe. set_solver.
+           }
+           apply storeA_union_swap_right. exact Hcompat_extra.
+Qed.
+
+End ResourceExtensionA.
+
+
+
+(** * Derived extension lemmas
+
+    This file is intentionally after the core extension files.  Long legacy proofs
+    that are really extension arguments should land here, not in the basic
+    resource files.  During the definition-migration phase these are named
+    review points. *)
+
+Section ResourceExtensionA.
+
+Context {K : Type} `{Countable K} .
+Context {V : Type} `{ValueSig V}.
+
+Local Notation StoreAT := (gmap K V) (only parsing).
+Local Notation WorldAT := (@WorldA K _ _ V) (only parsing).
+Local Notation WfWorldAT := (@WfWorldA K _ _ V) (only parsing).
+
+Lemma resA_extend_by_sum_pullback
+    (m : WfWorldAT) F (n n1 n2 : WfWorldAT)
+    (Hdef : rawA_sum_defined (n1 : WorldAT) (n2 : WorldAT)) :
+  resA_extend_by m F n →
+  fiber_extensionA_functional_on m F →
+  worldA_dom (m : WorldAT) ⊆ worldA_dom (n1 : WorldAT) →
+  worldA_dom (m : WorldAT) ⊆ worldA_dom (n2 : WorldAT) →
+  resA_sum n1 n2 Hdef ⊑ n →
+  ∃ (m1 m2 : WfWorldAT) (Hdefm : rawA_sum_defined m1 m2)
+    (n1' n2' : WfWorldAT),
+    worldA_dom (m1 : WorldAT) = worldA_dom (m : WorldAT) ∧
+    worldA_dom (m2 : WorldAT) = worldA_dom (m : WorldAT) ∧
+    resA_subset m1 m ∧
+    resA_subset m2 m ∧
+    resA_sum m1 m2 Hdefm ⊑ m ∧
+    resA_extend_by m1 F n1' ∧
+    n1 ⊑ n1' ∧
+    resA_extend_by m2 F n2' ∧
+    n2 ⊑ n2'.
+Proof.
+  intros Hext Hfun Hdom_m_n1 Hdom_m_n2 Hsum_le.
+  set (X := worldA_dom (m : WorldAT)).
+  set (m1 := resA_restrict n1 X).
+  set (m2 := resA_restrict n2 X).
+  assert (Hdom_m1 : worldA_dom (m1 : WorldAT) = X).
+  { subst m1 X. simpl. set_solver. }
+  assert (Hdom_m2 : worldA_dom (m2 : WorldAT) = X).
+  { subst m2 X. simpl. set_solver. }
+  assert (Hsub_m1_m : resA_subset m1 m).
+  {
+    subst m1 X.
+    split.
+    - simpl. set_solver.
+    - intros σ Hσ.
+      rewrite <- (resA_extend_by_restrict_base m F n Hext).
+      simpl in Hσ |- *.
+      destruct Hσ as [σ1 [Hσ1 Hrestrict1]].
+      unfold sqsubseteq, wf_worldA_sqsubseteq, resA_le, rawA_le in Hsum_le.
+      assert ((resA_sum n1 n2 Hdef : WorldAT) σ1) as Hsumσ1.
+      { simpl. left. exact Hσ1. }
+      rewrite Hsum_le in Hsumσ1. simpl in Hsumσ1.
+      destruct Hsumσ1 as [σn [Hσn Hrestrict_sum]].
+      exists σn. split; [exact Hσn |].
+      rewrite <- Hrestrict1, <- Hrestrict_sum.
+      rewrite storeA_restrict_restrict.
+      f_equal.
+      pose proof (rawA_le_dom _ _ Hsum_le) as Hdom_sum_n.
+      simpl in Hdom_sum_n.
+      rewrite Hdef in Hdom_sum_n.
+      set_solver.
+  }
+  assert (Hsub_m2_m : resA_subset m2 m).
+  {
+    subst m2 X.
+    split.
+    - simpl. set_solver.
+    - intros σ Hσ.
+      rewrite <- (resA_extend_by_restrict_base m F n Hext).
+      simpl in Hσ |- *.
+      destruct Hσ as [σ2 [Hσ2 Hrestrict2]].
+      unfold sqsubseteq, wf_worldA_sqsubseteq, resA_le, rawA_le in Hsum_le.
+      assert ((resA_sum n1 n2 Hdef : WorldAT) σ2) as Hsumσ2.
+      { simpl. right. exact Hσ2. }
+      rewrite Hsum_le in Hsumσ2. simpl in Hsumσ2.
+      destruct Hsumσ2 as [σn [Hσn Hrestrict_sum]].
+      exists σn. split; [exact Hσn |].
+      rewrite <- Hrestrict2, <- Hrestrict_sum.
+      rewrite storeA_restrict_restrict.
+      f_equal.
+      pose proof (rawA_le_dom _ _ Hsum_le) as Hdom_sum_n.
+      simpl in Hdom_sum_n.
+      set_solver.
+  }
+  assert (Hsub_m1_n : resA_subset m1 (resA_restrict n X)).
+  {
+    subst X. rewrite (resA_extend_by_restrict_base m F n Hext).
+    exact Hsub_m1_m.
+  }
+  assert (Hsub_m2_n : resA_subset m2 (resA_restrict n X)).
+  {
+    subst X. rewrite (resA_extend_by_restrict_base m F n Hext).
+    exact Hsub_m2_m.
+  }
+  set (n1' := resA_slice_restrict n X m1 Hsub_m1_n).
+  set (n2' := resA_slice_restrict n X m2 Hsub_m2_n).
+  assert (Hm1ext : resA_extend_by m1 F n1').
+  {
+    subst n1' X.
+    eapply resA_extend_by_slice_restrict_base; eauto.
+  }
+  assert (Hm2ext : resA_extend_by m2 F n2').
+  {
+    subst n2' X.
+    eapply resA_extend_by_slice_restrict_base; eauto.
+  }
+  assert (Hdefm : rawA_sum_defined (m1 : WorldAT) (m2 : WorldAT)).
+  { unfold rawA_sum_defined. rewrite Hdom_m1, Hdom_m2. reflexivity. }
+  exists m1, m2, Hdefm, n1', n2'.
+  split; [subst X; exact Hdom_m1 |].
+  split; [subst X; exact Hdom_m2 |].
+  split; [exact Hsub_m1_m |].
+  split; [exact Hsub_m2_m |].
+  refine (conj _ (conj Hm1ext (conj _ (conj Hm2ext _)))).
+  - subst m1 m2 X.
+    rewrite (resA_restrict_sum n1 n2 (worldA_dom (m : WorldAT)) Hdef Hdefm).
+    pose proof (resA_restrict_le_mono (resA_sum n1 n2 Hdef) n
+      (worldA_dom (m : WorldAT)) Hsum_le) as Hle_restrict.
+    rewrite (resA_extend_by_restrict_base m F n Hext) in Hle_restrict.
+    exact Hle_restrict.
+  - subst n1'. unfold sqsubseteq, wf_worldA_sqsubseteq, resA_le, rawA_le.
+    apply worldA_ext.
+    + simpl.
+      pose proof (rawA_le_dom _ _ Hsum_le) as Hdom_sum_n.
+      simpl in Hdom_sum_n. set_solver.
+    + intros σ. simpl. split.
+      * intros Hσ1.
+        unfold sqsubseteq, wf_worldA_sqsubseteq, resA_le, rawA_le in Hsum_le.
+        assert ((resA_sum n1 n2 Hdef : WorldAT) σ) as Hsumσ.
+        { simpl. left. exact Hσ1. }
+        rewrite Hsum_le in Hsumσ. simpl in Hsumσ.
+        destruct Hsumσ as [σn [Hσn Hrestrict]].
+        exists σn. split; [| exact Hrestrict].
+        split; [exact Hσn |].
+        subst m1. simpl.
+        exists σ. split; [exact Hσ1 |].
+        rewrite <- Hrestrict.
+        rewrite storeA_restrict_restrict.
+        replace (worldA_dom (n1 : WorldAT) ∩ X) with X by set_solver.
+        reflexivity.
+      * intros [σn [[Hσn Hσm1] Hrestrict]].
+        subst m1. simpl in Hσm1.
+        destruct Hσm1 as [σ1 [Hσ1 Hσ1_proj]].
+        unfold sqsubseteq, wf_worldA_sqsubseteq, resA_le, rawA_le in Hsum_le.
+        assert ((resA_sum n1 n2 Hdef : WorldAT) σ1) as Hsumσ1.
+        { simpl. left. exact Hσ1. }
+        rewrite Hsum_le in Hsumσ1. simpl in Hsumσ1.
+        destruct Hsumσ1 as [σn1 [Hσn1 Hrestrict1]].
+        apply (proj1 (resA_extend_by_store_iff _ _ _ _ Hext)) in Hσn.
+        apply (proj1 (resA_extend_by_store_iff _ _ _ _ Hext)) in Hσn1.
+        destruct Hσn as [σm [we [σe [Hσm [HFrel [Hσe Hσn_eq]]]]]].
+        destruct Hσn1 as [σm1 [we1 [σe1 [Hσm1 [HFrel1 [Hσe1 Hσn1_eq]]]]]].
+        subst σn σn1.
+        assert (Hbase :
+          @storeA_restrict V K _ _ (@union (gmap K V) _ σm σe) X = σm).
+        {
+          subst X.
+          exact (resA_extend_store_restrict_base m F σm we σe
+            (resA_extend_by_applicable _ _ _ Hext) Hσm HFrel Hσe).
+        }
+        assert (Hbase1 :
+          @storeA_restrict V K _ _ (@union (gmap K V) _ σm1 σe1) X = σm1).
+        {
+          subst X.
+          exact (resA_extend_store_restrict_base m F σm1 we1 σe1
+            (resA_extend_by_applicable _ _ _ Hext) Hσm1 HFrel1 Hσe1).
+        }
+        assert (Hσm1_eq : σm1 = σm).
+        {
+          rewrite <- Hbase1.
+          replace (@storeA_restrict V K _ _ (@union (gmap K V) _ σm1 σe1) X)
+            with (@storeA_restrict V K _ _ σ1 X).
+          2:{
+            rewrite <- Hrestrict1.
+            rewrite storeA_restrict_restrict.
+            replace (worldA_dom (resA_sum n1 n2 Hdef : WorldAT) ∩ X)
+              with X by (simpl; set_solver).
+            reflexivity.
+          }
+          rewrite Hσ1_proj.
+          exact Hbase.
+        }
+        subst σm1.
+        pose proof (fiber_extensionA_functional_outputs_eq m F σm we1 we σe1 σe
+          (resA_extend_by_applicable _ _ _ Hext) Hfun Hσm HFrel1 HFrel Hσe1 Hσe)
+          as Heq_fiber.
+        subst σe1.
+        rewrite Hrestrict1 in Hrestrict.
+        subst σ.
+        exact Hσ1.
+  - subst n2'. unfold sqsubseteq, wf_worldA_sqsubseteq, resA_le, rawA_le.
+    apply worldA_ext.
+    + simpl.
+      pose proof (rawA_le_dom _ _ Hsum_le) as Hdom_sum_n.
+      simpl in Hdom_sum_n |- *. rewrite <- Hdef. set_solver.
+    + intros σ. simpl. split.
+      * intros Hσ2.
+        unfold sqsubseteq, wf_worldA_sqsubseteq, resA_le, rawA_le in Hsum_le.
+        assert ((resA_sum n1 n2 Hdef : WorldAT) σ) as Hsumσ.
+        { simpl. right. exact Hσ2. }
+        rewrite Hsum_le in Hsumσ. simpl in Hsumσ.
+        destruct Hsumσ as [σn [Hσn Hrestrict]].
+        exists σn. split.
+        2:{ rewrite <- Hdef. exact Hrestrict. }
+        split; [exact Hσn |].
+        subst m2. simpl.
+        exists σ. split; [exact Hσ2 |].
+        rewrite <- Hrestrict.
+        rewrite storeA_restrict_restrict.
+        replace (worldA_dom (n1 : WorldAT) ∩ X) with X by set_solver.
+        reflexivity.
+      * intros [σn [[Hσn Hσm2] Hrestrict]].
+        subst m2. simpl in Hσm2.
+        destruct Hσm2 as [σ2 [Hσ2 Hσ2_proj]].
+        unfold sqsubseteq, wf_worldA_sqsubseteq, resA_le, rawA_le in Hsum_le.
+        assert ((resA_sum n1 n2 Hdef : WorldAT) σ2) as Hsumσ2.
+        { simpl. right. exact Hσ2. }
+        rewrite Hsum_le in Hsumσ2. simpl in Hsumσ2.
+        destruct Hsumσ2 as [σn2 [Hσn2 Hrestrict2]].
+        apply (proj1 (resA_extend_by_store_iff _ _ _ _ Hext)) in Hσn.
+        apply (proj1 (resA_extend_by_store_iff _ _ _ _ Hext)) in Hσn2.
+        destruct Hσn as [σm [we [σe [Hσm [HFrel [Hσe Hσn_eq]]]]]].
+        destruct Hσn2 as [σm2 [we2 [σe2 [Hσm2 [HFrel2 [Hσe2 Hσn2_eq]]]]]].
+        subst σn σn2.
+        assert (Hbase :
+          @storeA_restrict V K _ _ (@union (gmap K V) _ σm σe) X = σm).
+        {
+          subst X.
+          exact (resA_extend_store_restrict_base m F σm we σe
+            (resA_extend_by_applicable _ _ _ Hext) Hσm HFrel Hσe).
+        }
+        assert (Hbase2 :
+          @storeA_restrict V K _ _ (@union (gmap K V) _ σm2 σe2) X = σm2).
+        {
+          subst X.
+          exact (resA_extend_store_restrict_base m F σm2 we2 σe2
+            (resA_extend_by_applicable _ _ _ Hext) Hσm2 HFrel2 Hσe2).
+        }
+        assert (Hσm2_eq : σm2 = σm).
+        {
+          rewrite <- Hbase2.
+          replace (@storeA_restrict V K _ _ (@union (gmap K V) _ σm2 σe2) X)
+            with (@storeA_restrict V K _ _ σ2 X).
+          2:{
+            rewrite <- Hrestrict2.
+            rewrite storeA_restrict_restrict.
+            replace (worldA_dom (resA_sum n1 n2 Hdef : WorldAT) ∩ X)
+              with X by (simpl; rewrite Hdef; set_solver).
+            reflexivity.
+          }
+          rewrite Hσ2_proj.
+          exact Hbase.
+        }
+        subst σm2.
+        pose proof (fiber_extensionA_functional_outputs_eq m F σm we2 we σe2 σe
+          (resA_extend_by_applicable _ _ _ Hext) Hfun Hσm HFrel2 HFrel Hσe2 Hσe)
+          as Heq_fiber.
+        subst σe2.
+        assert (Hrestrict2' :
+          @storeA_restrict V K _ _ (@union (gmap K V) _ σm σe)
+            (worldA_dom (n2 : WorldAT)) = σ2).
+        {
+          rewrite <- Hdef. exact Hrestrict2.
+        }
+        rewrite Hrestrict2' in Hrestrict.
+        subst σ.
+        exact Hσ2.
+Qed.
+
+Lemma resA_one_point_extension_pushout
+    (m n my : WfWorldAT) (y : K) :
+  m ⊑ n →
+  y ∉ worldA_dom (n : WorldAT) →
+  worldA_dom (my : WorldAT) = worldA_dom (m : WorldAT) ∪ {[y]} →
+  resA_restrict my (worldA_dom (m : WorldAT)) = m →
+  ∃ ny : WfWorldAT,
+    worldA_dom (ny : WorldAT) = worldA_dom (n : WorldAT) ∪ {[y]} ∧
+    resA_restrict ny (worldA_dom (n : WorldAT)) = n ∧
+    my ⊑ ny.
+Proof.
+  intros Hmn Hy_n Hdom_my Hrestr_my.
+  pose proof (rawA_le_dom m n Hmn) as Hdom_m_n.
+  pose (raw_ny := ({|
+    worldA_dom := worldA_dom (n : WorldAT) ∪ {[y]};
+    worldA_stores := λ τ,
+      ∃ σn σy,
+        (n : WorldAT) σn ∧
+        (my : WorldAT) σy ∧
+        @storeA_restrict V K _ _ σn (worldA_dom (m : WorldAT)) =
+          @storeA_restrict V K _ _ σy (worldA_dom (m : WorldAT)) ∧
+        τ = @union (gmap K V) _ σn
+          (@storeA_restrict V K _ _ σy ({[y]} : gset K))
+  |} : WorldAT)).
+  assert (Hwf_ny : wf_worldA raw_ny).
+  {
+    constructor.
+    - destruct (wfA_ne _ (worldA_wf my)) as [σy Hσy].
+      assert (Hm_proj :
+          (m : WorldAT) (@storeA_restrict V K _ _ σy (worldA_dom (m : WorldAT)))).
+      {
+        assert (Hraw : rawA_restrict my (worldA_dom (m : WorldAT))
+            (@storeA_restrict V K _ _ σy (worldA_dom (m : WorldAT)))).
+        { exists σy. split; [exact Hσy | reflexivity]. }
+        assert (Heq : rawA_restrict my (worldA_dom (m : WorldAT)) = (m : WorldAT)).
+        {
+          change ((resA_restrict my (worldA_dom (m : WorldAT)) : WorldAT) =
+            (m : WorldAT)).
+          rewrite Hrestr_my. reflexivity.
+        }
+        rewrite Heq in Hraw. exact Hraw.
+      }
+      unfold sqsubseteq, wf_worldA_sqsubseteq, resA_le, rawA_le in Hmn.
+      rewrite Hmn in Hm_proj. simpl in Hm_proj.
+      destruct Hm_proj as [σn [Hσn Hrestrict]].
+      exists (@union (gmap K V) _ (σn : gmap K V)
+        (@storeA_restrict V K _ _ σy ({[y]} : gset K) : gmap K V)).
+      simpl. exists σn, σy. repeat split; eauto.
+      replace (worldA_dom (n : WorldAT) ∩ worldA_dom (m : WorldAT))
+        with (worldA_dom (m : WorldAT)) in Hrestrict by set_solver.
+      exact Hrestrict.
+    - intros τ [σn [σy [Hσn [Hσy [Hagree ->]]]]].
+      pose proof (wfworldA_store_dom n σn Hσn) as Hdomσn.
+      pose proof (wfworldA_store_dom my σy Hσy) as Hdomσy.
+      change (dom (σn : gmap K V) = worldA_dom (n : WorldAT)) in Hdomσn.
+      change (dom (σy : gmap K V) = worldA_dom (my : WorldAT)) in Hdomσy.
+      assert (Hcompat :
+          @storeA_compat V K _ _ σn (@storeA_restrict V K _ _ σy ({[y]} : gset K))).
+      {
+        apply storeA_disj_dom_compat.
+        apply set_eq. intros z. split.
+        - intros Hz.
+          apply elem_of_intersection in Hz as [Hzn Hzy].
+          change (z ∈ (dom (σn : gmap K V) : gset K)) in Hzn.
+          change (z ∈ (dom (@storeA_restrict V K _ _ σy ({[y]} : gset K) : gmap K V) : gset K)) in Hzy.
+          pose proof (storeA_restrict_dom σy ({[y]} : gset K)) as Hdom_restr.
+          change (dom (@storeA_restrict V K _ _ σy ({[y]} : gset K) : gmap K V) =
+            dom (σy : gmap K V) ∩ ({[y]} : gset K)) in Hdom_restr.
+          rewrite Hdom_restr in Hzy.
+          rewrite Hdomσn in Hzn.
+          apply elem_of_intersection in Hzy as [Hzy Hy].
+          change (z ∈ (dom (σy : gmap K V) : gset K)) in Hzy.
+          rewrite Hdomσy, Hdom_my in Hzy. set_solver.
+        - intros Hz. apply elem_of_empty in Hz. contradiction.
+      }
+      change (dom (@union (gmap K V) _ (σn : gmap K V)
+        (@storeA_restrict V K _ _ σy ({[y]} : gset K) : gmap K V)) =
+        worldA_dom (n : WorldAT) ∪ {[y]}).
+      rewrite (storeA_union_dom σn
+        (@storeA_restrict V K _ _ σy ({[y]} : gset K)) Hcompat).
+      pose proof (storeA_restrict_dom σy ({[y]} : gset K)) as Hdom_restr.
+      change (dom (@storeA_restrict V K _ _ σy ({[y]} : gset K) : gmap K V) =
+        dom (σy : gmap K V) ∩ ({[y]} : gset K)) in Hdom_restr.
+      rewrite Hdom_restr. rewrite Hdomσn.
+      apply set_eq. intros z. split.
+      * intros Hz.
+        apply elem_of_union in Hz as [Hz|Hz]; [set_solver |].
+        apply elem_of_intersection in Hz as [Hzy Hy].
+        change (z ∈ (dom (σy : gmap K V) : gset K)) in Hzy.
+        rewrite Hdomσy, Hdom_my in Hzy. set_solver.
+      * intros Hz.
+        apply elem_of_union.
+        destruct (decide (z ∈ worldA_dom (n : WorldAT))) as [Hzn|Hzn].
+        -- left. exact Hzn.
+        -- right. apply elem_of_intersection. split.
+           ++ change (z ∈ (dom (σy : gmap K V) : gset K)).
+              rewrite Hdomσy, Hdom_my. set_solver.
+           ++ set_solver.
+  }
+  exists (exist _ raw_ny Hwf_ny). split.
+  - reflexivity.
+  - split.
+    + apply wfworldA_ext. apply worldA_ext.
+      * simpl. set_solver.
+      * intros τ. simpl. split.
+        -- intros [τny [[σn [σy [Hσn [Hσy [Hagree ->]]]]] Hrestrict]].
+           rewrite (storeA_restrict_union_piece_l
+             σn (@storeA_restrict V K _ _ σy ({[y]} : gset K))
+             (worldA_dom (n : WorldAT)) ({[y]} : gset K)) in Hrestrict.
+           ++ subst τ. exact Hσn.
+           ++ apply storeA_compat_restrict_singleton_fresh.
+              pose proof (wfworldA_store_dom n σn Hσn) as Hdomσn.
+              change (dom (σn : gmap K V) = worldA_dom (n : WorldAT)) in Hdomσn.
+              change (y ∉ (dom (σn : gmap K V) : gset K)).
+              rewrite Hdomσn. exact Hy_n.
+           ++ pose proof (wfworldA_store_dom n σn Hσn) as Hdomσn.
+              change (dom (σn : gmap K V) = worldA_dom (n : WorldAT)) in Hdomσn.
+              intros z Hz. change (z ∈ (dom (σn : gmap K V) : gset K)) in Hz.
+              rewrite Hdomσn in Hz. exact Hz.
+           ++ apply storeA_restrict_dom_subset.
+           ++ set_solver.
+        -- intros Hτn.
+           assert (Hm_proj :
+               (m : WorldAT) (@storeA_restrict V K _ _ τ (worldA_dom (m : WorldAT)))).
+           {
+             unfold sqsubseteq, wf_worldA_sqsubseteq, resA_le, rawA_le in Hmn.
+             rewrite Hmn at 1. simpl. exists τ. split; [exact Hτn | reflexivity].
+           }
+           assert (Hraw_my :
+               rawA_restrict my (worldA_dom (m : WorldAT))
+                 (@storeA_restrict V K _ _ τ (worldA_dom (m : WorldAT)))).
+           {
+             assert (Heq : rawA_restrict my (worldA_dom (m : WorldAT)) = (m : WorldAT)).
+             {
+               change ((resA_restrict my (worldA_dom (m : WorldAT)) : WorldAT) =
+                 (m : WorldAT)).
+               rewrite Hrestr_my. reflexivity.
+             }
+             rewrite Heq. exact Hm_proj.
+           }
+           simpl in Hraw_my.
+           destruct Hraw_my as [σy [Hσy Hσy_restrict]].
+           exists (@union (gmap K V) _ (τ : gmap K V)
+             (@storeA_restrict V K _ _ σy ({[y]} : gset K) : gmap K V)).
+           split.
+           ++ simpl. exists τ, σy. repeat split; eauto.
+           ++ apply (storeA_restrict_union_piece_l
+                τ (@storeA_restrict V K _ _ σy ({[y]} : gset K))
+                (worldA_dom (n : WorldAT)) ({[y]} : gset K)).
+              ** apply storeA_compat_restrict_singleton_fresh.
+                 pose proof (wfworldA_store_dom n τ Hτn) as Hdomτ.
+                 change (dom (τ : gmap K V) = worldA_dom (n : WorldAT)) in Hdomτ.
+                 change (y ∉ (dom (τ : gmap K V) : gset K)).
+                 rewrite Hdomτ. exact Hy_n.
+              ** pose proof (wfworldA_store_dom n τ Hτn) as Hdomτ.
+                 change (dom (τ : gmap K V) = worldA_dom (n : WorldAT)) in Hdomτ.
+                 intros z Hz. change (z ∈ (dom (τ : gmap K V) : gset K)) in Hz.
+                 rewrite Hdomτ in Hz. exact Hz.
+              ** apply storeA_restrict_dom_subset.
+              ** set_solver.
+    + unfold sqsubseteq, wf_worldA_sqsubseteq, resA_le, rawA_le.
+      apply worldA_ext.
+      * simpl. rewrite Hdom_my. set_solver.
+      * intros τ. simpl. split.
+        -- intros Hτmy.
+           assert (Hm_proj :
+               (m : WorldAT) (@storeA_restrict V K _ _ τ (worldA_dom (m : WorldAT)))).
+           {
+             assert (Hraw : rawA_restrict my (worldA_dom (m : WorldAT))
+                 (@storeA_restrict V K _ _ τ (worldA_dom (m : WorldAT)))).
+             { exists τ. split; [exact Hτmy | reflexivity]. }
+             assert (Heq : rawA_restrict my (worldA_dom (m : WorldAT)) = (m : WorldAT)).
+             {
+               change ((resA_restrict my (worldA_dom (m : WorldAT)) : WorldAT) =
+                 (m : WorldAT)).
+               rewrite Hrestr_my. reflexivity.
+             }
+             rewrite Heq in Hraw. exact Hraw.
+           }
+           unfold sqsubseteq, wf_worldA_sqsubseteq, resA_le, rawA_le in Hmn.
+           rewrite Hmn in Hm_proj. simpl in Hm_proj.
+           destruct Hm_proj as [σn [Hσn Hrestrict]].
+           exists (@union (gmap K V) _ (σn : gmap K V)
+             (@storeA_restrict V K _ _ τ ({[y]} : gset K) : gmap K V)).
+           split.
+           ++ simpl. exists σn, τ. repeat split; eauto.
+              replace (worldA_dom (n : WorldAT) ∩ worldA_dom (m : WorldAT))
+                with (worldA_dom (m : WorldAT)) in Hrestrict by set_solver.
+              exact Hrestrict.
+           ++ pose proof (wfworldA_store_dom n σn Hσn) as Hdomσn.
+              pose proof (wfworldA_store_dom my τ Hτmy) as Hdomτ.
+              change (dom (σn : gmap K V) = worldA_dom (n : WorldAT)) in Hdomσn.
+              change (dom (τ : gmap K V) = worldA_dom (my : WorldAT)) in Hdomτ.
+              change (dom (σn : gmap K V) = worldA_dom (n : WorldAT)) in Hdomσn.
+              change (dom (τ : gmap K V) = worldA_dom (my : WorldAT)) in Hdomτ.
+              rewrite Hdom_my.
+              apply storeA_restrict_union_base_singleton.
+              ** intros z Hz. change (z ∈ (dom (σn : gmap K V) : gset K)).
+                 rewrite Hdomσn. apply Hdom_m_n. exact Hz.
+              ** change ((dom (τ : gmap K V) : gset K) =
+                   worldA_dom (m : WorldAT) ∪ {[y]}).
+                 rewrite Hdomτ, Hdom_my. reflexivity.
+              ** change (y ∉ (dom (σn : gmap K V) : gset K)).
+                 rewrite Hdomσn. exact Hy_n.
+              ** replace (worldA_dom (n : WorldAT) ∩ worldA_dom (m : WorldAT))
+                   with (worldA_dom (m : WorldAT)) in Hrestrict by set_solver.
+                 exact Hrestrict.
+        -- intros [τny [[σn [σy [Hσn [Hσy [Hagree ->]]]]] Hrestrict]].
+           rewrite Hdom_my in Hrestrict.
+           replace ((worldA_dom (n : WorldAT) ∪ {[y]}) ∩
+             (worldA_dom (m : WorldAT) ∪ {[y]}))
+             with (worldA_dom (m : WorldAT) ∪ {[y]}) in Hrestrict by set_solver.
+           change (@storeA_restrict V K _ _
+             (@union (gmap K V) _ σn (@storeA_restrict V K _ _ σy ({[y]} : gset K)))
+             (worldA_dom (m : WorldAT) ∪ {[y]}) = τ) in Hrestrict.
+           assert (Hglue :
+             @storeA_restrict V K _ _
+               (@union (gmap K V) _ σn (@storeA_restrict V K _ _ σy ({[y]} : gset K)))
+               (worldA_dom (m : WorldAT) ∪ {[y]}) = σy).
+           {
+             apply storeA_restrict_union_base_singleton.
+             - pose proof (wfworldA_store_dom n σn Hσn) as Hdomσn.
+               change (dom (σn : gmap K V) = worldA_dom (n : WorldAT)) in Hdomσn.
+               intros z Hz. change (z ∈ (dom (σn : gmap K V) : gset K)).
+               rewrite Hdomσn. apply Hdom_m_n. exact Hz.
+             - pose proof (wfworldA_store_dom my σy Hσy) as Hdomσy.
+               change (dom (σy : gmap K V) = worldA_dom (my : WorldAT)) in Hdomσy.
+               change ((dom (σy : gmap K V) : gset K) =
+                 worldA_dom (m : WorldAT) ∪ {[y]}).
+               rewrite Hdomσy, Hdom_my. reflexivity.
+             - pose proof (wfworldA_store_dom n σn Hσn) as Hdomσn.
+               change (dom (σn : gmap K V) = worldA_dom (n : WorldAT)) in Hdomσn.
+               change (y ∉ (dom (σn : gmap K V) : gset K)).
+               rewrite Hdomσn. exact Hy_n.
+             - exact Hagree.
+           }
+           rewrite Hglue in Hrestrict. subst τ. exact Hσy.
+Qed.
+
+End ResourceExtensionA.
