ContextTyping/theories/RegularDenotation.v
@@ -11,7 +11,7 @@
 From ContextTyping Require Export Typing.
 From ContextTyping Require Import Naming.
 From CoreLang Require Import BasicTyping.
-From ContextAlgebra Require Import ResourceInterfaceExtension.
+From ContextAlgebra Require Import ResourceInterface.
 From ContextBasicDenotation Require Import TermTLet.
 
 Definition denot_ty_regular_in_ctx_under
