ContextTyping/theories/TLetDenotation.v
@@ -8,7 +8,7 @@
     [Denotation.TLet.tlet_intro_denotation]. *)
 
 From CoreLang Require Import BasicTyping.
-From ContextAlgebra Require Import ResourceInterfaceExtension ResourceExtensionCore.
+From ContextAlgebra Require Import ResourceInterface ResourceExtension.
 From ContextBasicDenotation Require Import StoreTyping TermTLet Qualifier BasicTypingFormula.
 From Denotation Require Import ContextTypeDenotationSaturate.
 From ContextTyping Require Export TLetDirect.
