Denotation/theories/TLetSupport.v
@@ -4,7 +4,7 @@
 
 From Denotation Require Import Notation.
 From Denotation Require Import ContextTypeDenotationSaturate ContextTypeDenotationTactics.
-From ContextAlgebra Require Import ResourceAlgebraPullback.
+From ContextAlgebra Require Import ResourceAlgebra.
 From ContextLogic Require Import FormulaSyntaxTactics.
 From CoreLang Require Import InstantiationProps.
 From Stdlib Require Import List.
